## Solutions {-}

#### Solutions of Exercise 1. {-} 

(a) Deriving the upper bound: 
  $$
  \begin{align*}
  \frac{f(x)}{g(x|b)} 
  &= \frac{\frac{1}{\sqrt{2\pi}}\exp\left(-\frac{x^2}{2}\right)}{\frac{1}{2b}\exp\left(-\frac{|x|}{b}\right)}\\[2ex]
  &= \sqrt{\frac{2}{\pi}}\;b\; \exp\left(-\frac{x^2}{2}\right) \exp\left(\frac{|x|}{b}\right)\\[2ex]
  &= \sqrt{\frac{2}{\pi}}\;b\; \exp\left(\frac{2|x| - x^2b}{2b}\right)\\[2ex]
  &=\left\{
  \begin{array}{ll}
  \sqrt{\frac{2}{\pi}}\;b\; \exp\left(\frac{2 x  - x^2b}{2b}\right) &\;\text{for}\; x\geq 0\\
  \sqrt{\frac{2}{\pi}}\;b\; \exp\left(\frac{-2 x  - x^2b}{2b}\right) &\;\text{for}\; x <0,\\
  \end{array}
  \right.
  \end{align*}
  $$
  where $b>0.$ <br>
  First, consider the case of $x\geq 0.$ Maximizing  
  $$
  \begin{align*}
  \exp\left(\frac{2x - x^2b}{2b}\right) 
  & = \exp\left(\frac{1}{b}x - \frac{1}{2}x^2 \right)
  \end{align*}
  $$ 
  with respect to $x\geq 0$ yields
  $$
  \begin{align*}
  \exp\left(\frac{1}{b}x - \frac{1}{2}x^2 \right) \cdot \left(\frac{1}{b} - x \right) &\overset{!}{=} 0
  \Leftrightarrow 
  x=\frac{1}{b}
  \end{align*}
  $$ 
  Second, consider the case of $x<0.$ Maximizing 
  $$
  \begin{align*}
  \exp\left(\frac{-2x - x^2b}{2b}\right) 
  & = \exp\left(-\frac{1}{b}x - \frac{1}{2}x^2 \right)
  \end{align*}
  $$ 
  with respect to $x < 0$ yields
  $$
  \begin{align*}
  \exp\left(-\frac{1}{b}x - \frac{1}{2}x^2 \right) \cdot \left(-\frac{1}{b} - x \right) &\overset{!}{=} 0
  \Leftrightarrow 
  x=-\frac{1}{b}
  \end{align*}
  $$ 
  Thus
  $$
  \begin{align*}
  \frac{f(x)}{g(x|b)} 
  & \leq 
  %\left\{
  % \begin{array}{ll}
  % \sqrt{\frac{2}{\pi}}\;b\; \exp\left(\frac{2 \frac{1}{b}  - \frac{1}{b^2} b}{2b}\right) &\;\text{for}\; x\geq 0\\
  % \sqrt{\frac{2}{\pi}}\;b\; \exp\left(\frac{2 \frac{1}{b}  - \frac{1}{b^2} b}{2b}\right) &\;\text{for}\; x <0\\
  % \end{array}
  %\right.\\[2ex]
  \sqrt{\frac{2}{\pi}}\;b\; \exp\left(\frac{2 \frac{1}{b}  - \frac{1}{b} }{2b}\right) \\[2ex]
  &= 
  \sqrt{\frac{2}{\pi}}\;b\; \exp\left(\frac{1}{2b^2}\right)
  \end{align*}
  $$
  for $x\in\mathbb{R}.$ The following code produces a plot of the graph of 
  $$
  \frac{f(x)}{g(x|b)} = \sqrt{\frac{2}{\pi}}\;b\; \exp\left(\frac{2|x| - x^2b}{2b}\right)
  $$
  and marks the maximizing arguments $x=\pm 1/b$ for a given value of $b>0:$


```{r}
  b <- 1
  myfun <- function(x, b){sqrt(2/pi) * exp( (2*abs(x) - x^2 * b)/(2 * b) )}
  xx <- seq(-(1/b)*3, (1/b)*3, len = 500)
  yy <- myfun(xx, b = b)
  plot(x = xx, y = yy, type = "l")
  abline(v=c(-1/b, 1/b), lty=2)
```
  
  (b) To show that the minimum of the bound (in $b>0$) is attained at $b=1,$ we minimize 
$$
b\;\exp\left(\frac{1}{2b^2}\right)
$$
with respect to $b>0,$ which yields
$$
\begin{align*}
1\;\exp\left(\frac{1}{2b^2}\right) + b\;\exp\left(\frac{1}{2b^2}\right)\cdot \left(-2\frac{1}{2b^3}\right) &\overset{!}{=} 0\\[2ex]
1\; - 2\frac{1}{2b^2} &= 0\\[2ex]
b &= 1,
\end{align*}
$$
where we used that $\exp\left(\frac{1}{2b^2}\right)>0,$ which allows us to multiply both sides by $1/\exp\left(\frac{1}{2b^2}\right),$ and where the second solution $b=-1$ does not fulfill the requirement that $b>0.$ The following code produces a plot of the graph of 
$$
b\;\exp\left(\frac{1}{2b^2}\right).
$$


```{r}
myfun2 <- function(b){b * exp( 1/(2*b^2) )}
bb <- seq(.5, 2, len = 500)
yy <- myfun2(b = bb)
plot(x = bb, y = yy, type = "l")
abline(v = 1, lty=2)
```

#### Solutions of Exercise 2. {-}

$$
\begin{align*}
P\left(X \leq h (Y)\right)
&=\mathbb{E}\left(1_{(X \leq h (Y))}\right)\\[2ex]
&=\mathbb{E}\left[\mathbb{E}\left(1_{(X \leq h (Y))}|Y\right)    \right]\\[2ex]
&=\mathbb{E}\left[P\left(1_{(X \leq h (Y))}=1|Y\right)\cdot 1 + 0\right]\\[2ex]
&=\mathbb{E}\left[\;\;P\left(X \leq h (Y)|Y\right)\;\;\cdot\; 1\; + 0\right]\\[2ex]
&=\mathbb{E}\left[\;\;\int_{-\infty}^{h(Y)} f(x)dx \right]\\[2ex]
&=\mathbb{E}\left[\mathbb{E}\left[\left.\;\;\int_{-\infty}^{h(Y)} f(x)dx\right| Y \right]\right]\\[2ex]
&=\int_{-\infty}^{\infty} \;\;\left(\int_{-\infty}^{h (y)} f(x) dx \right) \quad g(y) dy
\end{align*}
$$


#### Solutions of Exercise 3. {-}

One can provide a graphical solution as following: 

![](images/Ch1_Exercise_Screenshot1.png)

Alternatively, one can do the following derivations:

$$
\begin{align*}
P\left(U\leq f_X(Y)\right)
&=\int_a^b\left(\int_0^{f_X(y)}\frac{1}{m}du\right)\frac{1}{b-a}dy\\[2ex]
&=\frac{1}{m}\cdot\frac{1}{b-a}\int_a^b\left(\int_0^{f_X(y)}\;1\;du\right)\;dy\\[2ex]
&=\frac{1}{m}\cdot\frac{1}{b-a}\int_a^b f_X(y) dy\\[2ex]
&=\frac{1}{m}\cdot\frac{1}{b-a}\cdot 1
\end{align*}
$$

#### Solutions of Exercise 4. {-} 

(a) Deriving the probability of accepting $Y$ from a simulation 
$$
(Y,U)\sim\mathcal{U}\left(\left\{(y,u)|y\in \operatorname{supp}(f_X)\;\text{and}\;0\leq u\leq Mg(y)\right\}\right).
$$ 
Since we accept $Y$ only if $U\leq f_X(Y),$
$$
\begin{align*}
P\left(\text{Accepting }Y\right)
&=P\left(U\leq f_X(Y)\right),
\end{align*}
$$
where $U\sim\mathcal{U}\left[0,Mg(Y)\right].$ <br>
Standardizing the uniform distribution yields
$$
\begin{align*}
P\left(\text{Accepting }Y\right)
&=P\left(\frac{U}{Mg(Y)}\leq \frac{f_X(Y)}{Mg(Y)}\right),\\[2ex]
\end{align*}
$$
where dividing by $Mg(Y)$ is allowed, since $Mg(y)>0$ for all $y\in\operatorname{supp}(f_X).$ <br>
Now, using that 
$$
\frac{U}{Mg(Y)} \sim\mathcal{U}\left[0,1\right],
$$ 
we have
$$
\begin{align*}
P\left(\text{Accepting }Y\right)
&=\int_{-\infty}^{\infty}\int_0^{\frac{f_X(y)}{Mg(y)}} 1 \; du\; g(y) \;dy\\[2ex] 
&=\int_{-\infty}^{\infty}\;\;\;\frac{f_X(y)}{Mg(y)}\;\; g(y) \;\;dy\\[2ex] 
&=\frac{1}{M}\int_{-\infty}^{\infty}\;f_X(y) \;\;dy\\[2ex] 
&=\frac{1}{M}
\end{align*}
$$
<!-- Note that this also is the ratio between the surface $\{\}$ of the subgraph of 
$$
\begin{align*}
\frac{1}{M} = \frac{\int f_X(y)dy}{\int M g(y)dy}
\end{align*}
$$ -->
(b) Showing that $M\geq 1:$
$$
  \begin{align*}
  f_X(x) & \leq M g(x)\quad \text{for all }\quad x\in\operatorname{supp}(f_X)\\[2ex]
  \int f_X(x) dx & \leq \int M g(x)dx = M \int  g(x)dx\\[2ex]
  1              & \leq M \cdot 1\\[2ex]
  \end{align*}
$$






<!-- 1.  If $U_1,\dots,U_n\overset{\text{i.i.d.}}{\sim}\mathcal{U}[0,1],$ then with $\mathbb{E}(U_1)=\mu=1/2$ and $\mathbb{V}(U_1)=\sigma^2=1/12,$
$$
\begin{align*}
Y_n
& =\frac{\sqrt{n}\left(\bar{U}_n - \mu\right)}{\sigma}\\[2ex]
& = \sqrt{12\; n}\left(\bar{U}_n - \frac{1}{2}\right) \\[2ex]
& \to_d \mathcal{N}(0,1).
\end{align*}
$$
  (a) Largest value $Y_n$ can take: 
     * Largest value $U_1$ can take is $1.$ 
     * Largest value $\bar{U}_n$ can take is $\frac{1}{n} n 1 = 1.$ 
     * Largest value $Y_n$ can take is $\sqrt{12\; n}\frac{1}{2}=\sqrt{3\;n}$
     By the same arguments, the smallest value $Y_n$ can take is $\sqrt{3\;n},$ thus the range of $Y_n$ is **bounded** for each given sample size $n,$ 
     $$
     Y_n\in\left[-\sqrt{3\; n}, \sqrt{3\; n}\right],
     $$
     while the standard normal distribution has **unbounded** range from $-\infty$ to $\infty$
  (b) Next, we derive the moments of $Y_n.$ 
     $$
     \begin{align*}
     M_{Y_n}(t) 
     & = \mathbb{E}\left(\exp\left(t Y_n \right)\right) \\[2ex] 
     & = \mathbb{E}\left(\exp\left(t \; \sqrt{12\; n}\left(\bar{U}_n - \frac{1}{2}\right)  \right)\right) \\[2ex] 
     & = \mathbb{E}\left(\exp\left(t \; \sqrt{12\; n}\left(\frac{1}{n}\sum_{i=1}^n U_i - \frac{1}{2}\right)  \right)\right) \\[2ex] 
     & = \mathbb{E}\left(\exp\left(t \; \sqrt{12\; n}\left(\frac{1}{n}\sum_{i=1}^n \left(U_i - \frac{1}{2}\right)\right)  \right)\right) \\[2ex] 
     & = \mathbb{E}\left(\exp\left( \frac{t \;\sqrt{12}}{\sqrt{n}}\sum_{i=1}^n \left(U_i - \frac{1}{2}\right)  \right)\right) \\[2ex] 
     & = \mathbb{E}\left(\exp\left( \sum_{i=1}^n \frac{t \;\sqrt{12}}{\sqrt{n}}\left(U_i - \frac{1}{2}\right)  \right)\right) \\[2ex] 
     & = \prod_{i=1}^n\mathbb{E}\left(\exp\left( \frac{t \;\sqrt{12}}{\sqrt{n}}\left(U_i - \frac{1}{2}\right)  \right)\right) \\[2ex] 
     & = \left(\mathbb{E}\left(\exp\left( \frac{t \;\sqrt{12}}{\sqrt{n}}\left(U_i - \frac{1}{2}\right)  \right)\right)\right)^n \\[2ex] 
     & = \left(\mathbb{E}\left(\exp\left( \frac{t U_i\;\sqrt{12}}{\sqrt{n}} - \frac{1}{2}\frac{t \;\sqrt{12}}{\sqrt{n}}  \right)\right)\right)^n \\[2ex]
     & = \left(\mathbb{E}\left(\exp\left( \frac{t U_i\;\sqrt{12}}{\sqrt{n}} + \frac{ - t \;\sqrt{3}}{\sqrt{n}}  \right)\right)\right)^n \\[2ex] 
     & = \left(\exp\left(\frac{ - t \;\sqrt{3}}{\sqrt{n}}\right)\right)^n
          \left(\mathbb{E}\left(\exp\left( \frac{t U_i\;\sqrt{12}}{\sqrt{n}}   \right)\right)\right)^n \\[2ex]
     & = \left(\exp\left(\frac{ - t \;\sqrt{3}}{\sqrt{n}}\right)\right)^n
          \left(\mathbb{E}\left(\exp\left( \frac{t \sqrt{12}}{\sqrt{n}} U_i   \right)\right)\right)^n \\[2ex] 
     & = \left(\exp\left(\frac{ - t \;\sqrt{3}}{\sqrt{n}}\right)\right)^n
          \left( \frac{\exp\left( \frac{t \sqrt{12}}{\sqrt{n}} -1 \right)}{\frac{t \sqrt{12}}{\sqrt{n}}}\right)^n \\[2ex] 
     & = \left(\exp\left(\frac{ - t \;\sqrt{3}}{\sqrt{n}}\right)\right)^n
          \left( \frac{t \sqrt{12}}{\sqrt{n}} \exp\left( \frac{t \sqrt{12}}{\sqrt{n}} -1 \right)\right)^n \\[2ex] 
     \end{align*}
     $$
     Since 
     $$
     M_U(t) = \mathbb{E}\left(\exp\left(t U\right)\right)=\frac{\exp(t) - 1}{t}.
     $$ 
     we also have  -->